Launchbury/HSemUpd.thy
@@ -14,72 +14,27 @@ begin
 
 definition HSem :: "('var \<times> 'exp) list \<Rightarrow> 'var f\<rightharpoonup> 'value \<rightarrow> 'var f\<rightharpoonup> 'value" 
   where
-  "HSem h = (\<Lambda> \<rho> . fix_on' (f\<emptyset>\<^bsub>[fdom \<rho> \<union> heapVars h]\<^esub>) (\<lambda> \<rho>'. \<rho> f++ heapToEnv h (\<lambda> e. \<lbrakk>e\<rbrakk>\<^bsub>\<rho>'\<^esub>)))"
+  "HSem \<Gamma> = (\<Lambda> \<rho> . (\<mu> \<rho>'. \<rho> f++\<^bsub>heapVars \<Gamma>\<^esub> heapToEnv \<Gamma> (\<lambda> e. \<lbrakk>e\<rbrakk>\<^bsub>\<rho>'\<^esub>)))"
 
 abbreviation HSem_syn ("\<lbrace> _ \<rbrace>_"  [60,60] 60) where "\<lbrace>\<Gamma>\<rbrace>\<rho> \<equiv> HSem \<Gamma> \<cdot> \<rho>"
 
-lemma fix_on_cond_HSem:
-  shows "fix_on_cond {x. f\<emptyset>\<^bsub>[fdom \<rho> \<union> heapVars h]\<^esub> \<sqsubseteq> x}
-          (f\<emptyset>\<^bsub>[fdom \<rho> \<union> heapVars h]\<^esub>) (\<lambda>\<rho>'. \<rho> f++ heapToEnv h (\<lambda>e. \<lbrakk>e\<rbrakk>\<^bsub>\<rho>'\<^esub>))"
-  apply (rule fix_on_condI)
-  apply (rule subpcpo_cone_above)
-  apply (rule bottom_of_cone_above)
-  apply (rule closed_onI, simp)
-  apply (rule cont_is_cont_on, simp)
-  done
-
-lemma HSem_monofun'': "monofun (\<lambda> \<rho>. fix_on' (f\<emptyset>\<^bsub>[fdom \<rho> \<union> heapVars \<Gamma>]\<^esub>) (\<lambda>\<rho>''. \<rho> f++ heapToEnv \<Gamma> (\<lambda>e. \<lbrakk> e \<rbrakk>\<^bsub>\<rho>''\<^esub>)))"
-  apply (rule monofunI)
-  apply (rule fix_on_mono2[OF fix_on_cond_HSem fix_on_cond_HSem])
-  unfolding fmap_below_dom[OF assms] apply rule
-  by (simp, intro fmap_add_mono assms heapToEnv_mono  cont2monofunE[OF cont2cont_heapToEnv] cont_Rep_cfun2)
-
-lemma HSem_cont'':
-  assumes "chain Y"
-  shows "fix_on' (f\<emptyset>\<^bsub>[fdom (\<Squnion> i. Y i) \<union> heapVars \<Gamma>]\<^esub>) (\<lambda>\<rho>'. (\<Squnion> i. Y i) f++ heapToEnv \<Gamma> (\<lambda>e. \<lbrakk> e \<rbrakk>\<^bsub>\<rho>'\<^esub>)) =
-        (\<Squnion> i. fix_on' (f\<emptyset>\<^bsub>[fdom (Y i) \<union> heapVars \<Gamma>]\<^esub>) (\<lambda>\<rho>'. Y i f++ heapToEnv \<Gamma> (\<lambda>e. \<lbrakk> e \<rbrakk>\<^bsub>\<rho>'\<^esub>)))"
-proof-
-  have fdoms:"\<And> i. fdom (Y i) = fdom (\<Squnion> i. Y i)" (is "\<And> _ .(_ = ?d)") by (metis chain_fdom `chain Y`) 
-  show ?thesis
-    unfolding fdoms
-    apply (rule fix_on_cont[OF `chain Y`, where S = "{x . f\<emptyset>\<^bsub>[fdom (\<Squnion> i. Y i) \<union> heapVars \<Gamma>]\<^esub> \<sqsubseteq> x}"])
-    apply (rule fix_on_cond_HSem[where \<rho> = "Y i", standard, where Y = Y, unfolded fdoms])
-    apply simp
-    done
-qed
-
-lemma HSem_cont':
-  shows "cont (\<lambda> \<rho>. fix_on' (f\<emptyset>\<^bsub>[fdom \<rho> \<union> heapVars \<Gamma>]\<^esub>) (\<lambda>\<rho>''. \<rho> f++ heapToEnv \<Gamma> (\<lambda>e. \<lbrakk> e \<rbrakk>\<^bsub>\<rho>''\<^esub>)))"
-  apply (rule contI2)
-  apply (rule HSem_monofun'')
-  apply (erule eq_imp_below[OF HSem_cont''])
-  done
-
 lemma HSem_def':
-    "\<lbrace>\<Gamma>\<rbrace>\<rho> = fix_on' (f\<emptyset>\<^bsub>[fdom \<rho> \<union> heapVars \<Gamma>]\<^esub>) (\<lambda> \<rho>'. \<rho> f++ heapToEnv \<Gamma> (\<lambda> e. \<lbrakk>e\<rbrakk>\<^bsub>\<rho>'\<^esub>))"
-  unfolding HSem_def
-  by (rule arg_cong[OF beta_cfun[OF HSem_cont']])
+    "\<lbrace>\<Gamma>\<rbrace>\<rho> = (\<mu> \<rho>'. \<rho> f++\<^bsub>heapVars \<Gamma>\<^esub> heapToEnv \<Gamma> (\<lambda> e. \<lbrakk>e\<rbrakk>\<^bsub>\<rho>'\<^esub>))"
+  unfolding HSem_def by simp
 
 subsubsection {* Induction and other lemmas about @{term HSem} *}
 
   lemma HSem_ind:
     assumes "adm P"
-    assumes "P (f\<emptyset>\<^bsub>[fdom \<rho> \<union> heapVars h]\<^esub>)"
-    assumes step: "\<And> y. fdom y = fdom \<rho> \<union> heapVars h \<Longrightarrow>
-          P y \<Longrightarrow>  P (\<rho> f++ (heapToEnv h (\<lambda>e. \<lbrakk>e\<rbrakk>\<^bsub>y\<^esub>)))"
-    shows "P (\<lbrace>h\<rbrace>\<rho>)"
+    assumes "P \<bottom>"
+    assumes step: "\<And> y. P y \<Longrightarrow>  P (\<rho> f++\<^bsub>heapVars \<Gamma>\<^esub> (heapToEnv \<Gamma> (\<lambda>e. \<lbrakk>e\<rbrakk>\<^bsub>y\<^esub>)))"
+    shows "P (\<lbrace>\<Gamma>\<rbrace>\<rho>)"
     unfolding HSem_def'
-    apply (rule fix_on_ind[OF fix_on_cond_HSem])
-    apply (rule adm_is_adm_on[OF `adm P`])
-    apply fact
-    apply (rule step)
-    apply simp
-    apply assumption
-    done
+    apply (rule fix_ind[OF assms(1,2)])
+    using step by simp
 
   lemma HSem_below:
-    assumes [simp]:"fdom r = fdom \<rho> \<union> heapVars h" 
-    assumes rho: "\<And>x. x \<in> fdom \<rho> \<Longrightarrow> x \<notin> heapVars h \<Longrightarrow> \<rho> f! x \<sqsubseteq> r f! x"
+    assumes rho: "\<And>x. x \<notin> heapVars h \<Longrightarrow> \<rho> f! x \<sqsubseteq> r f! x"
     assumes h: "\<And>x. x \<in> heapVars h \<Longrightarrow> \<lbrakk>the (map_of h x)\<rbrakk>\<^bsub>r\<^esub> \<sqsubseteq> r f! x"
     shows "\<lbrace>h\<rbrace>\<rho> \<sqsubseteq> r"
   proof (rule HSem_ind)
@@ -92,32 +47,26 @@ subsubsection {* Induction and other lemmas about @{term HSem} *}
   qed  
 
   lemma HSem_fempty_below:
-    assumes [simp]:"fdom r = heapVars h" 
     assumes h: "\<And>x. x \<in> heapVars h \<Longrightarrow> \<lbrakk>the (map_of h x)\<rbrakk>\<^bsub>r\<^esub> \<sqsubseteq> r f! x"
     shows "\<lbrace>h\<rbrace>f\<emptyset> \<sqsubseteq> r"
     using assms 
-    by (metis HSem_below fdomIff lookup_fempty subsetI sup.order_iff sup_commute)
+    by (metis HSem_below lookup_fempty minimal)
 
   lemma parallel_HSem_ind:
     assumes "adm (\<lambda>\<rho>'. P (fst \<rho>') (snd \<rho>'))"
-    assumes "P (f\<emptyset>\<^bsub>[fdom \<rho> \<union> heapVars h]\<^esub>) (f\<emptyset>\<^bsub>[fdom \<rho>2 \<union> heapVars h2]\<^esub>)"
-    assumes step: "\<And>y z. fdom y = fdom \<rho> \<union> heapVars h \<Longrightarrow>
-            fdom z = fdom \<rho>2 \<union> heapVars h2 \<Longrightarrow>
-            P y z \<Longrightarrow>
-            P (\<rho> f++ (heapToEnv h (\<lambda>e. \<lbrakk>e\<rbrakk>\<^bsub>y\<^esub>))) (\<rho>2 f++ (heapToEnv h2 (\<lambda>e. \<lbrakk>e\<rbrakk>\<^bsub>z\<^esub>)))"
-    shows "P (\<lbrace>h\<rbrace>\<rho>) (\<lbrace>h2\<rbrace>\<rho>2)"
+    assumes "P \<bottom> \<bottom>"
+    assumes step: "\<And>y z. P y z \<Longrightarrow>
+      P (\<rho> f++\<^bsub>heapVars \<Gamma>\<^esub> (heapToEnv \<Gamma> (\<lambda>e. \<lbrakk>e\<rbrakk>\<^bsub>y\<^esub>))) (\<rho>2 f++\<^bsub>heapVars \<Gamma>2\<^esub> (heapToEnv \<Gamma>2 (\<lambda>e. \<lbrakk>e\<rbrakk>\<^bsub>z\<^esub>)))"
+    shows "P (\<lbrace>\<Gamma>\<rbrace>\<rho>) (\<lbrace>\<Gamma>2\<rbrace>\<rho>2)"
     unfolding HSem_def'
-    apply (rule parallel_fix_on_ind[OF fix_on_cond_HSem fix_on_cond_HSem])
-    apply (rule adm_is_adm_on[OF `adm _`])
-    apply fact
-    apply (rule step)
-    apply simp+
-    done
+    find_theorems name:"fix" name:parallel
+    apply (rule parallel_fix_ind[OF assms(1,2)])
+    using step by simp
   
   lemma HSem_eq:
-    shows "\<lbrace>h\<rbrace>\<rho> = \<rho> f++ (heapToEnv h (\<lambda>e. \<lbrakk>e\<rbrakk>\<^bsub>\<lbrace>h\<rbrace>\<rho>\<^esub>))"
+    shows "\<lbrace>\<Gamma>\<rbrace>\<rho> = \<rho> f++\<^bsub>heapVars \<Gamma>\<^esub> (heapToEnv \<Gamma> (\<lambda>e. \<lbrakk>e\<rbrakk>\<^bsub>\<lbrace>\<Gamma>\<rbrace>\<rho>\<^esub>))"
     unfolding HSem_def'
-    by (rule fix_on_eq[OF fix_on_cond_HSem])  
+    by (subst fix_eq) simp
   
   lemma the_lookup_HSem_other:
     assumes "y \<notin> heapVars h"
@@ -125,27 +74,17 @@ subsubsection {* Induction and other lemmas about @{term HSem} *}
     apply (subst HSem_eq)
     using assms by simp
 
-  lemma fmap_lookup_bot_HSem_other:
-    assumes "y \<notin> heapVars h"
-    shows "(\<lbrace>h\<rbrace>\<rho>) f!\<^sub>\<bottom> y = \<rho> f!\<^sub>\<bottom> y"
-    using assms
-    by (subst HSem_eq, cases "y \<in> fdom \<rho>", auto)
-  
   lemma the_lookup_HSem_heap:
     assumes "y \<in> heapVars h"
     shows "(\<lbrace>h\<rbrace>\<rho>) f! y = \<lbrakk> the (map_of h y) \<rbrakk>\<^bsub>\<lbrace>h\<rbrace>\<rho>\<^esub>"
     apply (subst HSem_eq)
     using assms by (simp add: lookupHeapToEnv)
 
-  lemma fdom_HSem[simp]:
-    "fdom (\<lbrace>h\<rbrace>\<rho>) = fdom \<rho> \<union> heapVars h"
-    by (subst HSem_eq, simp)
-
-  lemma fmap_restr_fmap_addI:"fdom \<rho>1 - fdom \<rho>2 \<subseteq> S \<Longrightarrow> fmap_restr S \<rho>1 f++ \<rho>2 = \<rho>1 f++ \<rho>2"
+  lemma fmap_restr_fmap_addI:"-S2 \<subseteq> S \<Longrightarrow> fmap_restr S \<rho>1 f++\<^bsub>S2\<^esub> \<rho>2 = \<rho>1 f++\<^bsub>S2\<^esub> \<rho>2"
     by rule (auto simp add: lookup_fmap_add_eq)
 
   lemma HSem_restr:
-    "\<lbrace>h\<rbrace>(\<rho> f|` (fdom \<rho> - heapVars h)) = \<lbrace>h\<rbrace>\<rho>"
+    "\<lbrace>h\<rbrace>(\<rho> f|` (- heapVars h)) = \<lbrace>h\<rbrace>\<rho>"
     apply (rule parallel_HSem_ind)
     apply simp
     apply auto[1]
@@ -153,19 +92,10 @@ subsubsection {* Induction and other lemmas about @{term HSem} *}
     apply simp_all
     done
 
-  lemma HSem_restr':
-    "\<lbrace>h\<rbrace>(\<rho> f|` (- heapVars h)) = \<lbrace>h\<rbrace>\<rho>"
-    apply (rule parallel_HSem_ind)
-    apply simp
-    apply auto[1]
-    apply (subst fmap_restr_fmap_addI)
-    apply auto
-    done
-
   lemma HSem_fresh_cong:
     assumes "\<rho> f|` (- heapVars h) = \<rho>' f|` (- heapVars h)"
     shows "\<lbrace>h\<rbrace>\<rho> = \<lbrace>h\<rbrace>\<rho>'"
-    apply (subst (1 2) HSem_restr'[symmetric])
+    apply (subst (1 2) HSem_restr[symmetric])
     by (simp add: assms)
 
   lemma HSem_reorder:
@@ -197,9 +127,9 @@ subsubsection {* Induction and other lemmas about @{term HSem} *}
  lemma fmap_restr_HSem:
     assumes "heapVars \<Gamma> \<inter> S = {}"
     shows "fmap_restr S (\<lbrace>\<Gamma>\<rbrace>\<rho>) = fmap_restr S \<rho>"
-    apply (rule fmap_eqI)
-    using assms apply auto[1]
-    using assms apply auto[1]
+    apply rule
+    using assms 
+    apply (auto simp add: lookup_fmap_restr_eq)
     apply (subst the_lookup_HSem_other)
     apply auto
     done
@@ -209,11 +139,13 @@ subsubsection {* Induction and other lemmas about @{term HSem} *}
     shows "fmap_restr (fdom \<rho>) (\<lbrace>\<Gamma>\<rbrace>\<rho>) = \<rho>"
     by (simp add: fmap_restr_HSem[OF assms] fmap_restr_useless)
  
+  (*
   lemma HSem_disjoint_less:
     assumes "heapVars \<Gamma> \<inter> fdom \<rho> = {}"
     shows "\<rho> \<le> \<lbrace>\<Gamma>\<rbrace>\<rho>"
     using assms
   by (metis fmap_less_restrict fmap_restr_HSem_noop)
+  *)
 
   lemma HSem_Nil[simp]: "\<lbrace>[]\<rbrace>\<rho> = \<rho>"
     by (subst HSem_eq, simp)
@@ -224,24 +156,24 @@ subsubsection {* Re-calculating the semantics of the heap is idempotent *}
     shows "\<lbrace>\<Gamma>\<rbrace>(\<lbrace>\<Gamma> @ \<Delta>\<rbrace>\<rho>) f|` (fdom \<rho> \<union> heapVars \<Delta>) = \<lbrace>\<Gamma> @ \<Delta>\<rbrace>\<rho>" (is "?LHS = ?RHS")
   proof (rule below_antisym)
     show "?LHS \<sqsubseteq> ?RHS"
-    by (rule HSem_below) (auto simp add: the_lookup_HSem_heap)
-    
+    by (rule HSem_below)
+       (auto simp add: the_lookup_HSem_heap fmap_belowE[OF fmap_restr_below_itself])
+
   
     show "?RHS \<sqsubseteq> ?LHS"
     proof(rule HSem_below)
-    case goal1 show ?case by auto
+    case goal1
+      thus ?case
+      by (case_tac "x \<notin> fdom \<rho>") (auto simp add: the_lookup_HSem_other dest:lookup_not_fdom)
     next
-    case goal2
-      thus ?case by (auto simp add: the_lookup_HSem_other)
-    next
-    case (goal3 x)
+    case (goal2 x)
       thus ?case
       proof(cases "x \<in> heapVars \<Gamma>")
       case True
         thus ?thesis by (auto simp add: the_lookup_HSem_heap)
       next
       case False
-        hence delta: "x \<in> heapVars \<Delta>" using goal3 by auto
+        hence delta: "x \<in> heapVars \<Delta>" using goal2 by auto
         with False  `?LHS \<sqsubseteq> ?RHS`
         show ?thesis by (auto simp add: the_lookup_HSem_other the_lookup_HSem_heap monofun_cfun_arg)
       qed
@@ -253,9 +185,9 @@ subsubsection {* Iterative definition of the heap semantics *}
 
   lemma iterative_HSem:
     assumes "x \<notin> heapVars \<Gamma>"
-    shows "\<lbrace>(x,e) # \<Gamma>\<rbrace>\<rho> =
-         fix_on' (f\<emptyset>\<^bsub>[insert x (fdom \<rho> \<union> heapVars \<Gamma>)]\<^esub>)
-            (\<lambda> \<rho>'. (\<rho> f++ fmap_restr (heapVars \<Gamma>) (\<lbrace>\<Gamma>\<rbrace>\<rho>'))( x f\<mapsto> \<lbrakk>e\<rbrakk>\<^bsub>\<rho>'\<^esub>))"
+    shows "\<lbrace>(x,e) # \<Gamma>\<rbrace>\<rho> = (\<mu> \<rho>'. (\<rho> f++\<^bsub>heapVars \<Gamma>\<^esub> (\<lbrace>\<Gamma>\<rbrace>\<rho>'))( x f\<mapsto> \<lbrakk>e\<rbrakk>\<^bsub>\<rho>'\<^esub>))"
+  sorry
+  (*
   proof-
     interpret iterative
       where e1 =  "\<lambda> \<rho>'. heapToEnv \<Gamma> (\<lambda> e. \<lbrakk>e\<rbrakk>\<^bsub>\<rho>'\<^esub>)"
@@ -277,34 +209,14 @@ subsubsection {* Iterative definition of the heap semantics *}
       by (rule fix_on_cong[OF condR], simp add: HSem_def')
     finally show ?thesis.
   qed
-
-  lemma iterative_HSem'_cond:
-    assumes "x \<notin> heapVars \<Gamma>"
-    shows "fix_on_cond {\<rho>'. f\<emptyset>\<^bsub>[insert x (fdom \<rho> \<union> heapVars \<Gamma>)]\<^esub> \<sqsubseteq> \<rho>'}
-             (f\<emptyset>\<^bsub>[insert x (fdom \<rho> \<union> heapVars \<Gamma>)]\<^esub>)
-             (\<lambda> \<rho>'. (\<rho> f++ fmap_restr (heapVars \<Gamma>) (\<lbrace>\<Gamma>\<rbrace>\<rho>'))( x f\<mapsto> \<lbrakk>e\<rbrakk>\<^bsub>\<lbrace>\<Gamma>\<rbrace>\<rho>'\<^esub>))"
-  proof-
-    interpret iterative
-      where e1 =  "\<lambda> \<rho>'. heapToEnv \<Gamma> (\<lambda> e. \<lbrakk>e\<rbrakk>\<^bsub>\<rho>'\<^esub>)"
-      and e2 = "\<lambda> \<rho>'. \<lbrakk>e\<rbrakk>\<^bsub>\<rho>'\<^esub>"
-      and S = "heapVars \<Gamma>"
-      and x = x
-      and D =  "insert x (fdom \<rho> \<union> heapVars \<Gamma>) "
-      apply -
-      apply unfold_locales
-      using assms
-      by simp_all
-
-    show ?thesis
-      by (rule fix_on_cond_cong[OF condR'], simp add: HSem_def')
-  qed
+  *)
 
   lemma iterative_HSem':
     assumes "x \<notin> heapVars \<Gamma>"
-    shows "fix_on' (f\<emptyset>\<^bsub>[insert x (fdom \<rho> \<union> heapVars \<Gamma>)]\<^esub>)
-            (\<lambda> \<rho>'. (\<rho> f++ fmap_restr (heapVars \<Gamma>) (\<lbrace>\<Gamma>\<rbrace>\<rho>'))( x f\<mapsto> \<lbrakk>e\<rbrakk>\<^bsub>\<rho>'\<^esub>)) 
-       = fix_on' (f\<emptyset>\<^bsub>[insert x (fdom \<rho> \<union> heapVars \<Gamma>)]\<^esub>)
-            (\<lambda> \<rho>'. (\<rho> f++ fmap_restr (heapVars \<Gamma>) (\<lbrace>\<Gamma>\<rbrace>\<rho>'))( x f\<mapsto> \<lbrakk>e\<rbrakk>\<^bsub>\<lbrace>\<Gamma>\<rbrace>\<rho>'\<^esub>))"
+    shows "(\<mu> \<rho>'. (\<rho> f++\<^bsub>heapVars \<Gamma>\<^esub> (\<lbrace>\<Gamma>\<rbrace>\<rho>'))( x f\<mapsto> \<lbrakk>e\<rbrakk>\<^bsub>\<rho>'\<^esub>))
+         = (\<mu> \<rho>'. (\<rho> f++\<^bsub>heapVars \<Gamma>\<^esub> (\<lbrace>\<Gamma>\<rbrace>\<rho>'))( x f\<mapsto> \<lbrakk>e\<rbrakk>\<^bsub>\<lbrace>\<Gamma>\<rbrace>\<rho>'\<^esub>))"
+  sorry
+  (*
   proof-
     interpret iterative
       where e1 =  "\<lambda> \<rho>'. heapToEnv \<Gamma> (\<lambda> e. \<lbrakk>e\<rbrakk>\<^bsub>\<rho>'\<^esub>)"
@@ -331,6 +243,7 @@ subsubsection {* Iterative definition of the heap semantics *}
     finally
     show ?thesis.
   qed
+  *)
 
 end
 
@@ -347,13 +260,9 @@ lemma HSem_eqvt[eqvt]:
 proof-
   show ?thesis
    unfolding has_ESem.HSem_def
-   apply (subst permute_Lam[OF HSemUpd.has_ESem.HSem_cont'])
-   apply (rule arg_cong[where f = Abs_cfun])
+   apply (subst permute_Lam, simp)
    apply (subst eqvt_lambda)
-   apply rule
-   apply (subst fix_on_eqvt[OF has_ESem.fix_on_cond_HSem])
-   apply perm_simp
-   apply rule
+   apply (simp add: Cfun_app_eqvt permute_Lam)
    done
 qed
 
@@ -369,11 +278,9 @@ begin
     case adm thus ?case by simp
   next
     case base
-      from assms(1) heapVars_fv_subset have "heapVars \<Gamma> \<subseteq> S" by auto
-      thus ?case by -(rule, auto)
+      show ?case by simp
   next
     case (step y z)
-    thm step(3)[symmetric]
     have "heapToEnv \<Gamma> (\<lambda>e. \<lbrakk> e \<rbrakk>\<^bsub>y\<^esub>) = heapToEnv \<Gamma> (\<lambda>e. \<lbrakk> e \<rbrakk>\<^bsub>z\<^esub>)"
     proof(rule heapToEnv_cong')
       fix x
@@ -381,9 +288,11 @@ begin
       hence "fv (the (map_of \<Gamma> x)) \<subseteq> fv \<Gamma>" by (rule map_of_fv_subset)
       with assms(1)
       have "fv (the (map_of \<Gamma> x)) \<inter> S = fv (the (map_of \<Gamma> x))" by auto
+      with step
+      have "y f|` fv (the (map_of \<Gamma> x)) = z f|` fv (the (map_of \<Gamma> x))" by auto
       with `x \<in> heapVars \<Gamma>`
       show "\<lbrakk> the (map_of \<Gamma> x) \<rbrakk>\<^bsub>y\<^esub> = \<lbrakk> the (map_of \<Gamma> x) \<rbrakk>\<^bsub>z\<^esub>"
-        by (subst (1 2) assms(2)[OF `x \<in> heapVars \<Gamma>`]) (simp add: step(3)[symmetric])
+        by (subst (1 2) assms(2)[OF `x \<in> heapVars \<Gamma>`]) simp
     qed
     moreover
     have "heapVars \<Gamma> \<subseteq> S" using heapVars_fv_subset assms(1) by auto
@@ -416,12 +325,15 @@ begin
   proof-
     have "\<lbrakk> e \<rbrakk>\<^bsub>\<rho>\<^esub> =  \<lbrakk> e \<rbrakk>\<^bsub>\<rho> f|` (- (fdom \<rho> - S))\<^esub>"
       by (rule ESem_ignores_fresh_restr[OF assms])
-    also have "\<rho> f|` (- (fdom \<rho> - S)) = \<rho> f|` S" by auto
+    also have "\<rho> f|` (- (fdom \<rho> - S)) = \<rho> f|` S" 
+      by rule (auto simp add: lookup_fmap_restr_eq dest: lookup_not_fdom)
     finally show ?thesis.
   qed
 
+  (*
   lemma ESem_ignores_fresh: "\<rho>1 \<le> \<rho>2 \<Longrightarrow> atom ` (fdom \<rho>2 - fdom \<rho>1) \<sharp>* e \<Longrightarrow> \<lbrakk> e \<rbrakk>\<^bsub>\<rho>1\<^esub> = \<lbrakk> e \<rbrakk>\<^bsub>\<rho>2\<^esub>"
     by (metis ESem_ignores_fresh_restr' fmap_less_restrict)  
+  *)
 
   lemma HSem_ignores_fresh_restr:
     assumes "atom ` S \<sharp>* \<Gamma>"
@@ -436,43 +348,38 @@ subsubsection {* Adding a fresh variable to a heap does not affect its semantics
   lemma HSem_add_fresh':
     assumes fresh: "atom x \<sharp> \<Gamma>"
     assumes "x \<notin> fdom \<rho>"
-    assumes step: "\<And>e \<rho>'. fdom \<rho>' = fdom \<rho> \<union> heapVars ((x, e) # \<Gamma>) \<Longrightarrow> e \<in> snd ` set \<Gamma> \<Longrightarrow> \<lbrakk> e \<rbrakk>\<^bsub>\<rho>'\<^esub> = \<lbrakk> e \<rbrakk>\<^bsub>\<rho>' f|` (- {x})\<^esub>"
-    shows  "(\<lbrace>(x, e) # \<Gamma>\<rbrace>\<rho>) f|` (fdom \<rho> \<union> heapVars \<Gamma>) = \<lbrace>\<Gamma>\<rbrace>\<rho>"
+    assumes step: "\<And>e \<rho>'. e \<in> snd ` set \<Gamma> \<Longrightarrow> \<lbrakk> e \<rbrakk>\<^bsub>\<rho>'\<^esub> = \<lbrakk> e \<rbrakk>\<^bsub>fmap_delete x \<rho>'\<^esub>"
+    shows  "fmap_delete x (\<lbrace>(x, e) # \<Gamma>\<rbrace>\<rho>) = \<lbrace>\<Gamma>\<rbrace>\<rho>"
   proof (rule parallel_HSem_ind)
   case goal1 show ?case by simp
   case goal2 show ?case by auto
   case (goal3 y z)
-    have "fmap_restr (fdom \<rho> \<union> heapVars \<Gamma>) \<rho> = \<rho>" by auto
+    have "fmap_delete x \<rho> = \<rho>" using `x \<notin> fdom \<rho>` by (rule fmap_delete_noop)
     moreover
-    have "x \<notin> fdom \<rho> \<union> heapVars \<Gamma>"
-      using fresh `x \<notin> fdom \<rho>` by (auto simp add: fresh_Pair heapVars_not_fresh)
-    hence "fdom y \<inter> (- {x}) = fdom \<rho> \<union> heapVars \<Gamma>"
-      using goal3(1) by auto
-    hence [simp]: "z = y f|` (- {x})"
-      by (auto simp add: `_= z`[symmetric] intro: fmap_restr_cong)
-
-    have "heapToEnv ((x, e) # \<Gamma>) (\<lambda>e. \<lbrakk> e \<rbrakk>\<^bsub>y\<^esub>) f|` (fdom \<rho> \<union> heapVars \<Gamma>) = heapToEnv \<Gamma> (\<lambda>e. \<lbrakk> e \<rbrakk>\<^bsub>y\<^esub>)"
-      using `x \<notin> fdom \<rho> \<union> heapVars \<Gamma>` by auto
-    moreover
+    from fresh have "x \<notin> heapVars \<Gamma>" by (metis heapVars_not_fresh)
+    hence "fmap_delete x (heapToEnv ((x, e) # \<Gamma>) (\<lambda>e. \<lbrakk> e \<rbrakk>\<^bsub>y\<^esub>)) = heapToEnv \<Gamma> (\<lambda>e. \<lbrakk> e \<rbrakk>\<^bsub>y\<^esub>)"
+      by (auto intro: fmap_delete_noop dest:  set_mp[OF fdom_heapToEnv_subset])
+   moreover
     have "heapToEnv \<Gamma> (\<lambda>e. \<lbrakk> e \<rbrakk>\<^bsub>y\<^esub>) = heapToEnv \<Gamma> (\<lambda>e. \<lbrakk> e \<rbrakk>\<^bsub>z\<^esub>)"
       apply (rule heapToEnv_cong[OF refl])
-      apply (subst (1) step)
-      using goal3(1) apply auto
-      done
+      apply (subst (1) step, assumption)
+      using goal3(1) by auto
     ultimately
-    show ?case by (simp only: fmap_restr_add)
+    show ?case using `x \<notin> heapVars \<Gamma>`
+      by (simp add: fmap_delete_add)
   qed
 
   lemma HSem_add_fresh:
     assumes "atom x \<sharp> \<Gamma>"
     assumes "x \<notin> fdom \<rho>"
-    shows  "(\<lbrace>(x, e) # \<Gamma>\<rbrace>\<rho>) f|` (fdom \<rho> \<union> heapVars \<Gamma>) = \<lbrace>\<Gamma>\<rbrace>\<rho>"
+    shows  "fmap_delete x (\<lbrace>(x, e) # \<Gamma>\<rbrace>\<rho>) = \<lbrace>\<Gamma>\<rbrace>\<rho>"
   proof(rule HSem_add_fresh'[OF assms])
   case (goal1 e \<rho>')
     assume "e \<in> snd ` set \<Gamma>"
     hence "atom x \<sharp> e" by (metis assms(1) fresh_heap_expr')
-    hence "fv e \<inter> -{x} = fv e" by (auto simp add: fv_def fresh_def)
-    thus ?case by (simp cong: ESem_fresh_cong)
+    hence "x \<notin> fv e" by (simp add: fv_def fresh_def)
+    thus ?case 
+      by (rule ESem_fresh_cong[OF fmap_restr_fmap_delete_other[symmetric]])
   qed
  
 
@@ -482,17 +389,13 @@ subsubsection {* Binding more variables increases knowledge *}
     assumes fresh: "atom ` heapVars \<Gamma> \<sharp>* \<Delta>" 
     shows "\<lbrace>\<Delta>\<rbrace>(\<rho> f|` (- heapVars \<Gamma>)) \<sqsubseteq> (\<lbrace>\<Delta>@\<Gamma>\<rbrace>\<rho>)  f|` (- heapVars \<Gamma>)"
   proof(rule HSem_below)
-    from fresh
-    show "fdom ((\<lbrace>\<Delta> @ \<Gamma>\<rbrace>\<rho>) f|` (- heapVars \<Gamma>)) = fdom (\<rho> f|` (- heapVars \<Gamma>)) \<union> heapVars \<Delta>"
-      by (auto dest: fresh_distinct )
-
     fix x
     assume [simp]: "x \<in> heapVars \<Delta>"
     with assms have *: "atom ` heapVars \<Gamma> \<sharp>* the (map_of \<Delta> x)" by (metis fresh_star_map_of)
     hence [simp]: "x \<notin> heapVars \<Gamma>" using fresh `x \<in> heapVars \<Delta>` by (metis fresh_star_def heapVars_not_fresh image_eqI)
     show "\<lbrakk> the (map_of \<Delta> x) \<rbrakk>\<^bsub>(\<lbrace>\<Delta> @ \<Gamma>\<rbrace>\<rho>) f|` (- heapVars \<Gamma>)\<^esub> \<sqsubseteq> (\<lbrace>\<Delta> @ \<Gamma>\<rbrace>\<rho>) f|` (- heapVars \<Gamma>) f! x"
       by (simp add: the_lookup_HSem_heap ESem_ignores_fresh_restr[OF *, symmetric])
-   qed (simp add: the_lookup_HSem_other)
+   qed (simp add: the_lookup_HSem_other lookup_fmap_restr_eq)
 
   subsubsection {* Additional, fresh bindings in one or two steps *}  
 
@@ -519,7 +422,7 @@ subsubsection {* Binding more variables increases knowledge *}
     show "\<lbrace>\<Gamma>\<rbrace>\<lbrace>\<Delta>\<rbrace>\<rho> \<sqsubseteq> \<lbrace>\<Gamma>@\<Delta>\<rbrace>\<rho>"
     proof(rule HSem_below)
       fix x
-      assume "x \<in> fdom (\<lbrace>\<Delta>\<rbrace>\<rho>)" and [simp]:"x \<notin> heapVars \<Gamma>"
+      assume [simp]:"x \<notin> heapVars \<Gamma>"
 
       have "\<lbrace>\<Delta>\<rbrace>\<rho> f! x = ((\<lbrace>\<Delta>\<rbrace>\<rho>) f|` (- heapVars \<Gamma>)) f! x" by simp
       also have "\<dots> = \<lbrace>\<Delta>\<rbrace>(\<rho> f|` (- heapVars \<Gamma>)) f! x"
@@ -530,7 +433,7 @@ subsubsection {* Binding more variables increases knowledge *}
       also have "\<dots> = \<lbrace>\<Gamma> @ \<Delta>\<rbrace>\<rho>  f! x" by (rule arg_cong[OF HSem_reorder[OF map_of_eq]])
       finally
       show "\<lbrace>\<Delta>\<rbrace>\<rho> f! x \<sqsubseteq> \<lbrace>\<Gamma> @ \<Delta>\<rbrace>\<rho> f! x".
-    qed (auto simp add: the_lookup_HSem_heap)
+    qed (auto simp add: the_lookup_HSem_heap lookup_fmap_restr_eq)
 
      have *: "\<And> x. x \<in> heapVars \<Delta> \<Longrightarrow> x \<notin> heapVars \<Gamma>"
       using fresh by (auto simp add: fresh_Pair fresh_star_def heapVars_not_fresh)
@@ -558,6 +461,7 @@ subsubsection {* Binding more variables increases knowledge *}
 
   subsubsection {* The semantics of let only adds new bindings *}
   
+  (*
   lemma HSem_less:
     assumes fresh: "atom ` heapVars \<Gamma> \<sharp>* \<Delta>"
     assumes distinct: "heapVars \<Gamma> \<inter> fdom (\<lbrace>\<Delta>\<rbrace>\<rho>) = {}"
@@ -571,30 +475,20 @@ subsubsection {* Binding more variables increases knowledge *}
     finally
     show ?thesis.
   qed
+  *)
 
 subsubsection {* Substitution *}
 
   lemma HSem_subst_exp:
-    assumes "\<And>\<rho>'. fdom \<rho>' = fdom \<rho> \<union> (heapVars ((x,e)#\<Gamma>)) \<Longrightarrow>  \<lbrakk> e \<rbrakk>\<^bsub>\<rho>'\<^esub> = \<lbrakk> e' \<rbrakk>\<^bsub>\<rho>'\<^esub>"
+    assumes "\<And>\<rho>'. \<lbrakk> e \<rbrakk>\<^bsub>\<rho>'\<^esub> = \<lbrakk> e' \<rbrakk>\<^bsub>\<rho>'\<^esub>"
     shows "\<lbrace>(x, e) # \<Gamma>\<rbrace>\<rho> = \<lbrace>(x, e') # \<Gamma>\<rbrace>\<rho>"
     by (rule parallel_HSem_ind) (auto simp add: assms heapToEnv_subst_exp)
 
   lemma HSem_subst_expr_below:
     assumes below: "\<lbrakk> e1 \<rbrakk>\<^bsub>\<lbrace>(x, e2) # \<Gamma>\<rbrace>\<rho>\<^esub> \<sqsubseteq> \<lbrakk> e2 \<rbrakk>\<^bsub>\<lbrace>(x, e2) # \<Gamma>\<rbrace>\<rho>\<^esub>"
     shows "\<lbrace>(x, e1) # \<Gamma>\<rbrace>\<rho> \<sqsubseteq> \<lbrace>(x, e2) # \<Gamma>\<rbrace>\<rho>"
-  proof (rule HSem_ind) back
-  case goal1 show ?case by auto
-  case goal2 show ?case by (simp add: to_bot_fmap_def)
-  case (goal3 \<rho>')
-    show ?case
-      apply (subst HSem_eq)
-      apply (rule fmap_add_mono[OF below_refl])
-      apply simp
-      apply (rule fmap_upd_mono)
-      apply (rule cont2monofunE[OF cont2cont_heapToEnv[OF cont_Rep_cfun2] goal3(2)])
-      apply (rule below_trans[OF cont2monofunE[OF cont_Rep_cfun2 goal3(2)] below])
-      done
-  qed
+  by (rule HSem_below) (auto simp add: the_lookup_HSem_heap below to_bot_fmap_def the_lookup_HSem_other)
+
   
   lemma HSem_subst_expr:
     assumes below1: "\<lbrakk> e1 \<rbrakk>\<^bsub>\<lbrace>(x, e2) # \<Gamma>\<rbrace>\<rho>\<^esub> \<sqsubseteq> \<lbrakk> e2 \<rbrakk>\<^bsub>\<lbrace>(x, e2) # \<Gamma>\<rbrace>\<rho>\<^esub>"
@@ -606,8 +500,8 @@ end
 
 lemma parallel_HSem_ind_different_ESem:
   assumes "adm (\<lambda>\<rho>'. P (fst \<rho>') (snd \<rho>'))"
-  assumes "P (f\<emptyset>\<^bsub>[fdom \<rho> \<union> heapVars h]\<^esub>) (f\<emptyset>\<^bsub>[fdom \<rho>2 \<union> heapVars h2]\<^esub>)"
-  assumes "\<And>y z. P y z \<Longrightarrow> P (\<rho> f++ heapToEnv h (\<lambda>e. ESem1 e $ y)) (\<rho>2 f++ heapToEnv h2 (\<lambda>e. ESem2 e $ z))"
+  assumes "P f\<emptyset> f\<emptyset>"
+  assumes "\<And>y z. P y z \<Longrightarrow> P (\<rho> f++\<^bsub>heapVars h\<^esub> heapToEnv h (\<lambda>e. ESem1 e $ y)) (\<rho>2 f++\<^bsub>heapVars h2\<^esub> heapToEnv h2 (\<lambda>e. ESem2 e $ z))"
   shows "P (has_ESem.HSem ESem1 h\<cdot>\<rho>) (has_ESem.HSem ESem2 h2\<cdot>\<rho>2)"
 proof-
   interpret HSem1: has_ESem ESem1.
@@ -615,9 +509,10 @@ proof-
 
   show ?thesis
     unfolding HSem1.HSem_def' HSem2.HSem_def'
-    apply (rule parallel_fix_on_ind[OF HSem1.fix_on_cond_HSem HSem2.fix_on_cond_HSem])
-    apply (rule adm_is_adm_on[OF assms(1)])
+    apply (rule parallel_fix_ind[OF assms(1)])
+    unfolding bot_is_fmap_empty
     apply (rule assms(2))
+    apply simp
     apply (erule assms(3))
     done
 qed
