Launchbury/HeapToEnv.thy
@@ -6,9 +6,9 @@ default_sort type
 
 subsubsection {* Conversion from heaps to environments *} 
 
-function heapToEnv :: "('var \<times> 'exp) list \<Rightarrow> ('exp \<Rightarrow> 'value) \<Rightarrow> 'var f\<rightharpoonup> 'value"
+function heapToEnv :: "('var \<times> 'exp) list \<Rightarrow> ('exp \<Rightarrow> 'value::pcpo) \<Rightarrow> 'var f\<rightharpoonup> 'value"
 where
-  "heapToEnv [] _ = fempty"
+  "heapToEnv [] _ = f\<emptyset>"
 | "heapToEnv ((x,e)#h) eval = (heapToEnv h eval) (x f\<mapsto> eval e)"
 by (pat_completeness, auto)
 termination by lexicographic_order
@@ -21,12 +21,8 @@ lemma heapToEnv_eqvt[eqvt]:
   "\<pi> \<bullet> heapToEnv h eval = heapToEnv (\<pi> \<bullet> h) (\<pi> \<bullet> eval)"
   by (induct h eval rule:heapToEnv.induct, auto simp add: fmap_upd_eqvt)
 
-lemma heapToEnv_fdom[simp]:"fdom (heapToEnv h eval) = heapVars h"
-  by (induct h eval rule:heapToEnv.induct, auto)
-
-lemma fmap_restr_heapToEnv_noop:
-  "heapVars h \<subseteq> S \<Longrightarrow> fmap_restr S (heapToEnv h eval) = heapToEnv h eval"
-  by rule auto
+lemma fdom_heapToEnv_subset:"fdom (heapToEnv h eval) \<subseteq> heapVars h"
+  by (induct h eval rule:heapToEnv.induct) (auto dest:set_mp[OF fdom_fmap_upd_subset])
 
 lemma heapToEnv_cong[fundef_cong]:
   "\<lbrakk> heap1 = heap2 ;  (\<And> e. e \<in> snd ` set heap2 \<Longrightarrow> eval1 e = eval2 e) \<rbrakk>
@@ -43,16 +39,38 @@ lemma lookupHeapToEnv:
   apply auto
   done
 
+lemma lookupHeapToEnv_other[simp]:
+  assumes "v \<notin> heapVars h"
+  shows "(heapToEnv h f) f! v = \<bottom>"
+  using assms
+  apply (induct h)
+  apply simp
+  apply (case_tac a)
+  apply auto
+  done
+
+
+lemma fmap_restr_heapToEnv_noop:
+  "heapVars h \<subseteq> S \<Longrightarrow> fmap_restr S (heapToEnv h eval) = heapToEnv h eval"
+  apply rule
+  apply (case_tac "x \<in> S")
+  apply (auto simp add: lookupHeapToEnv intro: lookupHeapToEnv_other)
+  done
+
 lemma heapToEnv_cong':
   "\<lbrakk> (\<And> x. x \<in> heapVars heap \<Longrightarrow> eval1 (the (map_of heap x)) = eval2 (the (map_of heap x))) \<rbrakk>
     \<Longrightarrow>  heapToEnv heap eval1 = heapToEnv heap eval2"
- by rule (auto simp add: lookupHeapToEnv)
+ apply rule
+ apply (case_tac "x \<in> heapVars heap")
+ apply (auto simp add: lookupHeapToEnv)
+ done
 
 lemma lookupHeapToEnvNotAppend[simp]:
   assumes "x \<notin> heapVars \<Gamma>"
   shows "heapToEnv (\<Gamma>@h) f f! x = heapToEnv h f f! x"
   using assms by (induct \<Gamma>, auto)
 
+(*
 lemma heapToEnv_remove_Cons_fmap_expand:
   "finite S \<Longrightarrow> x \<notin> S \<Longrightarrow> heapToEnv ((x, e) # \<Gamma>) eval\<^bsub>[S]\<^esub> = heapToEnv \<Gamma> eval\<^bsub>[S]\<^esub>"
   apply (rule fmap_eqI)
@@ -63,21 +81,19 @@ lemma heapToEnv_remove_Cons_fmap_expand:
   apply simp
   apply auto
   done
+*)
 
 lemma heapToEnv_delete[simp]: "heapToEnv (delete x \<Gamma>) eval = fmap_delete x (heapToEnv \<Gamma> eval)"
   by (induct \<Gamma>) auto
 
 lemma heapToEnv_mono:
-  "finite d1 \<Longrightarrow>
-   d1 = d2 \<Longrightarrow>
-   x \<notin> heapVars \<Gamma> \<Longrightarrow>
-  heapToEnv \<Gamma> eval\<^bsub>[d1]\<^esub> \<sqsubseteq> heapToEnv ((x, e) # \<Gamma>) eval\<^bsub>[d2]\<^esub>"
-   apply (erule subst)
-   apply (rule fmap_expand_belowI)
+  "x \<notin> heapVars \<Gamma> \<Longrightarrow>
+  heapToEnv \<Gamma> eval \<sqsubseteq> heapToEnv ((x, e) # \<Gamma>) eval"
    apply simp
-   apply (rule eq_imp_below)
-   apply simp
-   apply (metis lookup_fmap_upd_other[symmetric])
+   apply (rule fmap_belowI)
+   apply (case_tac "xa \<in> heapVars \<Gamma>")
+   apply (case_tac "xa = x")
+   apply auto
    done
 
 subsubsection {* Reordering lemmas *}
@@ -88,13 +104,13 @@ lemma heapToEnv_reorder:
 proof (rule fmap_eqI)
   from assms
   have *: "heapVars \<Gamma> = heapVars \<Delta>" by (metis dom_map_of_conv_heapVars)
-  thus "fdom (heapToEnv \<Gamma> h) = fdom (heapToEnv \<Delta> h)" by simp
-  
+
   fix x
-  assume "x \<in> fdom (heapToEnv \<Gamma> h)"
-  hence "x \<in> heapVars \<Gamma>" "x \<in> heapVars \<Delta>" using * by simp_all
-  thus "heapToEnv \<Gamma> h f! x = heapToEnv \<Delta> h f! x" using assms(1)
-    by (simp add: lookupHeapToEnv)
+  show "heapToEnv \<Gamma> h f! x = heapToEnv \<Delta> h f! x" 
+    using assms(1) *
+    apply (cases "x \<in> heapVars \<Gamma>")
+    apply (auto simp add: lookupHeapToEnv)
+    done
 qed
 
 lemma heapToEnv_reorder_head:
