Launchbury/Denotational-Related.thy
@@ -2,22 +2,14 @@ theory "Denotational-Related"
 imports "Denotational" "ResourcedDenotational" ValueSimilarity
 begin
 
-theorem
+theorem denotational_semantics_similar: 
   assumes "\<rho> f\<triangleleft>\<triangleright> \<sigma>"
-  shows denotational_semantics_similar: "\<lbrakk>e\<rbrakk>\<^bsub>\<rho>\<^esub> \<triangleleft>\<triangleright> (\<N>\<lbrakk>e\<rbrakk>\<^bsub>\<sigma>\<^esub>)\<cdot>(C\<^sup>\<infinity>)"
+  shows "\<lbrakk>e\<rbrakk>\<^bsub>\<rho>\<^esub> \<triangleleft>\<triangleright> (\<N>\<lbrakk>e\<rbrakk>\<^bsub>\<sigma>\<^esub>)\<cdot>(C\<^sup>\<infinity>)"
 using assms
 proof(induct e arbitrary: \<rho> \<sigma> rule:exp_induct)
   case (Var v)
-  show ?case
-  proof (cases "v \<in> fdom \<rho>")
-    case False
-    with Var have "v \<notin> fdom \<sigma>" by cases auto
-    thus ?thesis using False by simp
-  next
-    case True
-    with Var have "\<rho> f!\<^sub>\<bottom> v \<triangleleft>\<triangleright> (\<sigma> f!\<^sub>\<bottom> v)\<cdot>C\<^sup>\<infinity>" by cases auto
-    thus ?thesis by simp
-  qed
+  hence "\<rho> f! v \<triangleleft>\<triangleright> (\<sigma> f! v)\<cdot>C\<^sup>\<infinity>" by cases auto
+  thus ?case by simp
 next
   case (Lam v e)
   { fix x y
@@ -38,26 +30,19 @@ next
   next
     case (Fn f g)
     from `\<rho> f\<triangleleft>\<triangleright> \<sigma>`
-    have "\<rho> f!\<^sub>\<bottom> v \<triangleleft>\<triangleright> (\<sigma> f!\<^sub>\<bottom> v)\<cdot>C\<^sup>\<infinity>"  by auto
+    have "\<rho> f! v \<triangleleft>\<triangleright> (\<sigma> f! v)\<cdot>C\<^sup>\<infinity>"  by auto
     thus ?thesis using Fn App' by auto
   qed
 next
   case (Let as e \<rho> \<sigma>)
-  have "fdom \<rho> = fdom \<sigma>" using Let(3) by auto
-
   have "\<lbrace>asToHeap as\<rbrace>\<rho> f\<triangleleft>\<triangleright> \<N>\<lbrace>asToHeap as\<rbrace>\<sigma>"
-  proof (rule parallel_HSem_ind_different_ESem[OF fmap_similar_adm])
-    case goal1 show ?case by (simp add: `fdom \<rho> = fdom \<sigma>`)
-  next
-    case (goal2 \<rho>' \<sigma>')
+  proof (rule parallel_HSem_ind_different_ESem[OF fmap_similar_adm fmap_similar_fmap_bottom])
+    case (goal1 \<rho>' \<sigma>')
     show ?case
     proof(rule fmap_lift_relI)
-      case goal1 show ?case by (simp add:  `fdom \<rho> = fdom \<sigma>`)
-    next
-      case (goal2 x)
-      hence "x \<in> fdom \<rho> \<and> x \<notin> heapVars (asToHeap as) \<or> x \<in> heapVars (asToHeap as)" by auto
-      thus ?case using `\<rho>' f\<triangleleft>\<triangleright> \<sigma>'` `\<rho> f\<triangleleft>\<triangleright> \<sigma>`
-        by (auto simp add: lookupHeapToEnv elim: Let(1) )
+      case (goal1 x)
+      show ?case using `\<rho> f\<triangleleft>\<triangleright> \<sigma>`
+        by (auto simp add: lookup_fmap_add_eq lookupHeapToEnv elim: Let(1)[OF _  `\<rho>' f\<triangleleft>\<triangleright> \<sigma>'`] )
     qed
   qed
   with Let(2)
@@ -67,6 +52,6 @@ qed
 
 theorem heaps_similar: "\<lbrace>\<Gamma>\<rbrace> f\<triangleleft>\<triangleright> \<N>\<lbrace>\<Gamma>\<rbrace>"
   by (rule parallel_HSem_ind_different_ESem[OF fmap_similar_adm])
-     (auto simp add: lookupHeapToEnv denotational_semantics_similar)
+     (auto simp add: lookup_fmap_restr_eq lookupHeapToEnv denotational_semantics_similar)
 
 end
