Launchbury/Env-Nominal.thy
@@ -1,13 +1,13 @@
 theory "Env-Nominal"
-  imports Env "Nominal-Utils"
+  imports Env "Nominal-Utils" "Nominal-HOLCF"
 begin
 
 subsubsection {* Permtuations on finite maps *}
 
-instantiation "fmap" :: (pt,pt) pt
+instantiation "fmap" :: (pt,pcpo_pt) pt
 begin
-  lift_definition permute_fmap :: "perm \<Rightarrow> 'a::pt f\<rightharpoonup> 'b::pt \<Rightarrow> 'a f\<rightharpoonup> 'b"
-    is "\<lambda> p f . p \<bullet> f" by (metis (full_types) dom_perm_rev permute_finite)
+  lift_definition permute_fmap :: "perm \<Rightarrow> 'a f\<rightharpoonup> 'b \<Rightarrow> 'a f\<rightharpoonup> 'b"
+    is "\<lambda> p f . p \<bullet> f" ..
   
   instance
   apply(default)
@@ -21,57 +21,40 @@ lemma lookup_eqvt[eqvt]:
   "\<pi> \<bullet> lookup m x = lookup (\<pi> \<bullet> m) (\<pi> \<bullet> x)"
   by transfer simp
 
-lemma the_lookup_eqvt:
-  "x \<in> fdom m \<Longrightarrow> \<pi> \<bullet> (m f! x) = (\<pi> \<bullet> m) f! (\<pi> \<bullet> x)"
-  apply (transfer fixing: x) 
-  apply auto
-  by (metis Some_eqvt permute_fun_app_eq the.simps)
-
 lemma the_lookup_perm[simp]:
-  fixes \<rho> :: "'a::at_base f\<rightharpoonup> 'b::pure"
+  fixes \<rho> :: "'a::at_base f\<rightharpoonup> 'b::{pure,pcpo_pt}"
   shows "((x' \<leftrightarrow> x) \<bullet> \<rho>) f! xa = \<rho> f! ((x' \<leftrightarrow> x) \<bullet> xa) " 
   by (metis lookup_eqvt permute_flip_cancel permute_pure)
 
 lemma fempty_eqvt[eqvt, simp]:
-  "\<pi> \<bullet> fempty = fempty"
-  by (transfer, auto simp add: permute_fun_def)
+  "\<pi> \<bullet> f\<emptyset> = f\<emptyset>"
+  by transfer auto
 
-lemma fempty_supp[simp]: "supp fempty = {}"
-  by (metis eqvtI fempty_eqvt supp_fun_eqvt)
+lemma fempty_supp[simp]: "supp f\<emptyset> = {}"
+  by (metis eqvt_def fempty_eqvt supp_fun_eqvt)
 
-lemma fempty_fresh[simp]: "a \<sharp> fempty"
+lemma fempty_fresh[simp]: "a \<sharp> f\<emptyset>"
   by (simp add: fresh_def)
 
-lemma fempty_fresh_star[simp]: "a \<sharp>* fempty"
+lemma fempty_fresh_star[simp]: "a \<sharp>* f\<emptyset>"
   by (simp add: fresh_star_def)
 
 lemma fdom_perm: "fdom (\<pi> \<bullet> f) = \<pi> \<bullet> (fdom f)"
-  apply transfer by (rule dom_perm)
+  by transfer auto
+
 lemmas fdom_perm_rev[simp,eqvt] = fdom_perm[symmetric]
 
 lemma mem_fdom_perm[simp]:
-  fixes \<rho> :: "'a::at_base f\<rightharpoonup> 'b::pure"
+  fixes \<rho> :: "'a::at_base f\<rightharpoonup> 'b::{pcpo_pt}"
   shows "xa \<in> fdom (p \<bullet> \<rho>) \<longleftrightarrow> - p \<bullet> xa \<in> fdom \<rho>" 
   by (metis (mono_tags) fdom_perm_rev mem_Collect_eq permute_set_eq)
 
 lemma fmap_upd_eqvt[eqvt]: "p \<bullet> (fmap_upd f x y) = fmap_upd (p \<bullet> f) (p \<bullet> x) (p \<bullet> y)"
-  by transfer (metis Some_eqvt fun_upd_eqvt)
+  by transfer (metis fun_upd_eqvt)
 
 lemma fmap_restr_eqvt[eqvt]:
-  "\<pi> \<bullet> (fmap_restr d m) = fmap_restr (\<pi> \<bullet> d) (\<pi> \<bullet> m)"
-proof
-case goal1 thus ?case by (metis fdom_fmap_restr fdom_perm_rev inter_eqvt)
-case goal2
-  from goal2 have "x \<in> \<pi> \<bullet> fdom m \<inter> \<pi> \<bullet> d" by (metis (full_types) fdom_fmap_restr fdom_perm_rev inter_eqvt)
-  then obtain y where "x = \<pi> \<bullet> y" and "y \<in> fdom m \<inter> d" by (auto simp add: permute_set_def)
-
-  have "(\<pi> \<bullet> fmap_restr d m) f! x = (\<pi> \<bullet> fmap_restr d m) f! (\<pi> \<bullet> y)" by (simp add: `x = _`)
-  also have "... = \<pi> \<bullet> ((fmap_restr d m) f! y)" using  `y \<in> fdom m \<inter> d` by (metis fdom_fmap_restr the_lookup_eqvt)
-  also have "... = \<pi> \<bullet> (m f! y)" using `y \<in> _` by simp
-  also have "... = (\<pi> \<bullet> m) f! x" using `x = _` `y \<in> _` by (simp add: the_lookup_eqvt)
-  also have "... = fmap_restr (\<pi> \<bullet> d) (\<pi> \<bullet> m) f! x" using `x \<in> _ \<inter> _` by simp
-  finally show ?case.
-qed
+  "\<pi> \<bullet> m f|` d = (\<pi> \<bullet> m) f|` (\<pi> \<bullet> d)"
+  by transfer auto
 
 lemma fmap_delete_eqvt[eqvt]:
   "\<pi> \<bullet> fmap_delete x m = fmap_delete (\<pi> \<bullet> x) (\<pi> \<bullet> m)"
@@ -82,12 +65,14 @@ lemma fmap_copy_eqvt[eqvt]:
   by transfer simp
 
 lemma fmap_add_eqvt[eqvt]:
-  "\<pi> \<bullet> m1 f++ m2 = (\<pi> \<bullet> m1) f++ (\<pi> \<bullet> m2)"
+  "\<pi> \<bullet> m1 f++\<^bsub>S\<^esub> m2 = (\<pi> \<bullet> m1) f++\<^bsub>\<pi> \<bullet> S\<^esub> (\<pi> \<bullet> m2)"
   by transfer simp
 
+(*
 lemma fmap_of_eqvt[eqvt]:
   "\<pi> \<bullet> fmap_of l = fmap_of (\<pi> \<bullet> l)"
-by transfer (rule map_of_eqvt)
+  by transfer (rule map_of_eqvt)
+*)
 
 lemma fmap_map_eqvt[eqvt]:
   "\<pi> \<bullet> fmap_map f m = fmap_map (\<pi> \<bullet> f) (\<pi> \<bullet> m)"
@@ -96,7 +81,7 @@ by transfer simp
 subsubsection {* Permutation and restriction *}
 
 lemma fmap_restr_perm:
-  fixes \<rho> :: "'a::at f\<rightharpoonup> 'b::pure"
+  fixes \<rho> :: "'a::at_base f\<rightharpoonup> 'b::{pcpo_pt,pure}"
   assumes "supp p \<sharp>* S" and [simp]: "finite S"
   shows "(p \<bullet> \<rho>) f|` S = \<rho> f|` S"
 using assms
@@ -111,10 +96,13 @@ apply (auto simp add:perm_supp_eq supp_minus_perm fresh_star_def fresh_def supp_
 done
 
 lemma fmap_restr_flip:
-  fixes \<rho> :: "'a::at f\<rightharpoonup> 'b::pure"
+  fixes \<rho> :: "'a::at f\<rightharpoonup> 'b::{pcpo_pt,pure}"
   assumes "x \<notin> S" and "x' \<notin> S"
   shows "((x' \<leftrightarrow> x) \<bullet> \<rho>) f|` S = \<rho> f|` S"
   using assms
-  by (auto simp add: permute_flip_at  split:if_splits)
+  apply transfer
+  apply rule
+  apply (auto  simp add: permute_flip_at split:if_splits)
+  by (metis eqvt_lambda flip_at_base_simps(3) minus_flip permute_pure unpermute_def)
 
 end
