Launchbury/ResourcedDenotational.thy
@@ -16,16 +16,16 @@ abbreviation HSem_fempty  ("\<N>\<lbrace>_\<rbrace>"  [60] 60) where "\<N>\<lbra
 (* The same, but with some beta_cfun's and eta_cfuns resolved.*)
 lemma CESem_simps:
   "\<N>\<lbrakk> Lam [x]. e \<rbrakk>\<^bsub>\<rho>\<^esub> = (\<Lambda> (C\<cdot>r). (CFn\<cdot>(\<Lambda> v. C_restr\<cdot>r\<cdot>(\<N>\<lbrakk>e\<rbrakk>\<^bsub>\<rho>(x f\<mapsto> C_restr\<cdot>r\<cdot>v)\<^esub>))))"
-  "\<N>\<lbrakk> App e x \<rbrakk>\<^bsub>\<rho>\<^esub>    = (\<Lambda> (C\<cdot>r). ((\<N>\<lbrakk>e\<rbrakk>\<^bsub>\<rho>\<^esub>)\<cdot>r \<down>CFn C_restr\<cdot>r\<cdot>(\<rho> f!\<^sub>\<bottom> x))\<cdot>r)"
-  "\<N>\<lbrakk> Var x \<rbrakk>\<^bsub>\<rho>\<^esub>      = (\<Lambda> (C\<cdot>r). (\<rho> f!\<^sub>\<bottom> x) \<cdot> r)"
+  "\<N>\<lbrakk> App e x \<rbrakk>\<^bsub>\<rho>\<^esub>    = (\<Lambda> (C\<cdot>r). ((\<N>\<lbrakk>e\<rbrakk>\<^bsub>\<rho>\<^esub>)\<cdot>r \<down>CFn C_restr\<cdot>r\<cdot>(\<rho> f! x))\<cdot>r)"
+  "\<N>\<lbrakk> Var x \<rbrakk>\<^bsub>\<rho>\<^esub>      = (\<Lambda> (C\<cdot>r). (\<rho> f! x) \<cdot> r)"
   "\<N>\<lbrakk> Let as body \<rbrakk>\<^bsub>\<rho>\<^esub> = (\<Lambda> (C \<cdot> r). (\<N>\<lbrakk>body\<rbrakk>\<^bsub>\<N>\<lbrace>asToHeap as\<rbrace>\<rho>\<^esub>) \<cdot> r)"
   by (simp_all)
 
 lemma CESem_bot[simp]:"(\<N>\<lbrakk> e \<rbrakk>\<^bsub>\<sigma>\<^esub>)\<cdot>\<bottom> = \<bottom>"
   by (nominal_induct e arbitrary: \<sigma> rule: exp_assn.strong_induct(1)) auto
 
-lemma CHSem_bot[simp]:"(\<N>\<lbrace> \<Gamma> \<rbrace> f!\<^sub>\<bottom> x)\<cdot> \<bottom> = \<bottom>"
-  by (cases "x \<in> heapVars \<Gamma>") (auto simp add: the_lookup_HSem_heap)
+lemma CHSem_bot[simp]:"(\<N>\<lbrace> \<Gamma> \<rbrace> f! x)\<cdot> \<bottom> = \<bottom>"
+  by (cases "x \<in> heapVars \<Gamma>") (auto simp add: the_lookup_HSem_heap the_lookup_HSem_other)
 
 end
 
